Cleaned a bit

ntor/Security.ec
@@ -88,7 +88,7 @@ clone Split as ROc with
   type from        <= pkey * pkey * s_id * pkey * pkey,
   type to          <= tag * key,
   op   sampleto  _ <= dtag `*` dkey,
-  type input       <= unit,
+  type input       <= bool,
   type output      <= bool
 proof *.
 
@@ -104,7 +104,7 @@ realize topairK by rewrite /topair /ofpair.
 realize ofpairK by rewrite /topair /ofpair.
 realize sample_spec by rewrite /ofpair dprodC dmap_comp //=.
 
-module (Red_ROM_real (D : A_GAKE) : ROc.IdealAll.RO_Distinguisher) (O : ROc.IdealAll.RO) = {
+module (Red_ROM (D : A_GAKE) : ROc.IdealAll.RO_Distinguisher) (O : ROc.IdealAll.RO) = {
   module AKE_O : GAKE_out = Game1 with {
     proc h [ 
       ^tk<$ ~ {tk <@ O.get(x);}
@@ -112,34 +112,15 @@ module (Red_ROM_real (D : A_GAKE) : ROc.IdealAll.RO_Distinguisher) (O : ROc.Idea
     ] res ~ (tk)
   }
 
-  proc distinguish() = {
+  proc distinguish(b) = {
     var b';
-    AKE_O.init_mem(false);
+    AKE_O.init_mem(b);
     b' <@ D(AKE_O).run();
     return b';
   }
 }.
 
-module (Red_ROM_ideal (D : A_GAKE) : ROc.IdealAll.RO_Distinguisher) (O : ROc.IdealAll.RO) = {
-  module AKE_O : GAKE_out = Game1 with {
-    proc h [ 
-      ^tk<$ ~ {tk <@ O.get(x);}
-      ^if -
-    ] res ~ (tk)
-  }
-
-  proc distinguish() = {
-    var b';
-    AKE_O.init_mem(true);
-    b' <@ D(AKE_O).run();
-    return b';
-  }
-}.
-
-
-print Game2.
-
-module (Red_ROM2_real (D : A_GAKE) (O1 : ROSc.I1.RO) : ROSc.I2.RO_Distinguisher) (O2 : ROSc.I2.RO) = {
+module (Red_ROM2 (D : A_GAKE) (O1 : ROSc.I1.RO) : ROSc.I2.RO_Distinguisher) (O2 : ROSc.I2.RO) = {
   module AKE_O : GAKE_out = Game2 with {
     proc init_mem [
       ^h1m<- ~ {O1.init();}
@@ -188,75 +169,13 @@ module (Red_ROM2_real (D : A_GAKE) (O1 : ROSc.I1.RO) : ROSc.I2.RO_Distinguisher)
     ]
   }
 
-  proc distinguish() = {
-    var b;
-    AKE_O.init_mem(false);
-    b <@ D(AKE_O).run();
-    return b;
+  proc distinguish(b) = {
+    var b';
+    AKE_O.init_mem(b);
+    b' <@ D(AKE_O).run();
+    return b';
   }
 }.
-
-print Red_ROM2_real.AKE_O.
-
-
-module (Red_ROM2_ideal (D : A_GAKE) (O1 : ROSc.I1.RO) : ROSc.I2.RO_Distinguisher) (O2 : ROSc.I2.RO) = {
-  module AKE_O : GAKE_out = Game2 with {
-    proc init_mem [
-      ^h1m<- ~ {O1.init();}
-      ^h2m<- -
-    ]
-
-    proc h [ 
-      ^t<$ ~ {t <@ O1.get(x); k <@ O2.get(x);}
-      ^if -
-      ^k<$ -
-      ^if -
-    ] res ~ ((t, k))
-
-    proc send_msg2 [
-      ^match#Some.^match#None.^if.^ts<$ ~ {t_B <@ O1.get(x); O2.sample(x); sk <- witness;}
-      [^match#Some.^match#None.^if.^if - ^sk<-] -
-    ]
-
-    proc send_msg3 [
-      ^match#Some.^match#Pending.^ts<$ ~ {t_A <@ O1.get(x); O2.sample(x); sk <- witness;}
-      [^match#Some.^match#Pending.^if - ^sk<-] -
-    ]
-
-    proc c_rev_skey [
-      var ks : key
-      var x : pkey * pkey * s_id * pkey * pkey
-      ^match#Some.^match#Accepted.^if.^k<- ~ {x <- ((oget t'.`2).`1 ^ st'.`4, st'.`2 ^ st'.`4, st'.`1, st'.`3, (oget t'.`2).`1); ks <@ O2.get(x); k <- Some ks;}
-    ]
-
-    proc s_rev_skey [
-      var ks : key
-      var x : pkey * pkey * s_id * pkey * pkey
-      ^match#Some.^match#Accepted.^if.^k<- ~ {x <- (t'.`1 ^ (oget st'.`3), t'.`1 ^ st'.`2, st'.`1, t'.`1, (oget t'.`2).`1); ks <@ O2.get(x); k <- Some ks;}
-    ]
-
-    proc c_test [
-      var ks2 : key
-      ^if.^match#Some.^match#Accepted.^if.^if.^k<- ~ {ks <@ O2.get(x); k <- Some ks;}
-      ^if.^match#Some.^match#Accepted.^if.^if?^ks<$ + ^ {ks2 <@ O2.get(x);}
-    ]
-
-    proc s_test [
-      var ks2 : key
-      ^if.^match#Some.^match#Accepted.^if.^if.^k<- ~ {ks <@ O2.get(x); k <- Some ks;}
-      ^if.^match#Some.^match#Accepted.^if.^if?^ks<$ + ^ {ks2 <@ O2.get(x);}
-    ]
-  }
-
-  proc distinguish() = {
-    var b;
-    AKE_O.init_mem(true);
-    b <@ D(AKE_O).run();
-    return b;
-  }
-}.
-
-print Red_ROM2_ideal.AKE_O.
 
 
 (* ------------------------------------------------------------------------------------------ *)
@@ -264,7 +183,7 @@ print Red_ROM2_ideal.AKE_O.
 (* ------------------------------------------------------------------------------------------ *)
 section.
 
-declare module A <: A_GAKE {-GAKEb, -Game0, -Game1, -Game2, -Game3, -ROc.IdealAll.RO, -RO, -FRO, -ROSc.I1.RO, -ROSc.I2.RO, -ROSc.I1.FRO, -ROSc.I2.FRO, -Red_Coll_real, -Red_Coll_ideal, -BB.Sample, -Red_ROM_real, -Red_ROM_ideal, -Red_ROM2_real, -Red_ROM2_ideal }.
+declare module A <: A_GAKE {-GAKEb, -Game0, -Game1, -Game2, -Game3, -ROc.IdealAll.RO, -RO, -FRO, -ROSc.I1.RO, -ROSc.I2.RO, -ROSc.I1.FRO, -ROSc.I2.FRO, -Red_Coll_real, -Red_Coll_ideal, -BB.Sample, -Red_ROM, -Red_ROM2 }.
 
 declare axiom A_ll (G <: GAKE_out{-A}):
   islossless G.h =>
@@ -829,15 +748,13 @@ proof *.
 
 lemma game1_game2 bit &m: Pr[E_GAKE(Game1, A).run(bit) @ &m : res] =  Pr[E_GAKE(Game2, A).run(bit) @ &m : res].
 proof.
-case (bit = false) => real_ideal.
-
 (* Proof on the real side *)
-byequiv (: ={glob A, glob Red_ROM_real} /\ arg{1} = bit /\ arg{2} = bit ==> _) => //.
+byequiv (: ={glob A, glob Red_ROM} /\ arg{1} = bit /\ arg{2} = bit ==> _) => //.
 proc*.
-transitivity*  {1} { r <@ ROc.IdealAll.MainD(Red_ROM_real(A), ROc.IdealAll.RO).distinguish(); }.
+transitivity*  {1} { r <@ ROc.IdealAll.MainD(Red_ROM(A), ROc.IdealAll.RO).distinguish(bit); }.
 
 + inline; wp.
-  call (: ={b0, servers, c_smap, s_smap, tested, kp_set, bad}(Game1, Red_ROM_real.AKE_O) /\ Game1.hm{1} = ROc.IdealAll.RO.m{2}); 
+  call (: ={b0, servers, c_smap, s_smap, tested, kp_set, bad}(Game1, Red_ROM.AKE_O) /\ Game1.hm{1} = ROc.IdealAll.RO.m{2}); 
     try sim />.
 
   + proc; inline.
@@ -862,11 +779,11 @@ transitivity*  {1} { r <@ ROc.IdealAll.MainD(Red_ROM_real(A), ROc.IdealAll.RO).d
 
   + auto.
 
-transitivity*  {2} { r <@ ROc.IdealAll.MainD(Red_ROM_real(A), ROSc.RO_Pair(ROSc.I1.RO,ROSc.I2.RO)).distinguish(); };
-  1: by call (ROSc.RO_split (Red_ROM_real(A))).
+transitivity*  {2} { r <@ ROc.IdealAll.MainD(Red_ROM(A), ROSc.RO_Pair(ROSc.I1.RO,ROSc.I2.RO)).distinguish(bit); };
+  1: by call (ROSc.RO_split (Red_ROM(A))).
 
 inline; wp.
-call (: ={b0, servers, c_smap, s_smap, tested, kp_set, bad}(Red_ROM_real.AKE_O, Game2) /\ Game2.h1m{2} = ROSc.I1.RO.m{1} /\ Game2.h2m{2} = ROSc.I2.RO.m{1}
+call (: ={b0, servers, c_smap, s_smap, tested, kp_set, bad}(Red_ROM.AKE_O, Game2) /\ Game2.h1m{2} = ROSc.I1.RO.m{1} /\ Game2.h2m{2} = ROSc.I2.RO.m{1}
           /\ forall x, x \in ROSc.I1.RO.m{1} <=> x \in ROSc.I2.RO.m{1}); 
     try sim />.
 
@@ -878,71 +795,6 @@ call (: ={b0, servers, c_smap, s_smap, tested, kp_set, bad}(Red_ROM_real.AKE_O, 
   smt(mem_set).
 
 + proc; inline.
-  sp 2 2; match = => // sk.
-  match = => //.
-  seq 1 1: (#pre /\ ={kp}); 1: by auto.
-  sp 1 1; if => //.
-  sp. seq 1 1: (#pre /\ r0{1} = ts{2}); 1: by auto => />.
-  auto => />.
-  smt(mem_set).
-
-+ proc; inline.
-  sp 1 1; match = => // st.
-  match = => // st' pt ir.
-  sp. seq 1 1: (#pre /\ r0{1} = ts{2}); 1: by auto.
-  auto => />.
-  smt(mem_set).
-
-auto => />.
-smt(emptyE).
-
-(* Proof on the ideal side *)
-byequiv (: ={glob A, glob Red_ROM_ideal} /\ arg{1} = bit /\ arg{2} = bit ==> _) => //.
-proc*.
-transitivity*  {1} { r <@ ROc.IdealAll.MainD(Red_ROM_ideal(A), ROc.IdealAll.RO).distinguish(); }.
-
-+ inline; wp.
-  call (: ={b0, servers, c_smap, s_smap, tested, kp_set, bad}(Game1, Red_ROM_ideal.AKE_O) /\ Game1.hm{1} = ROc.IdealAll.RO.m{2}); 
-    try sim />.
-
-  + proc; inline.
-    case ((x \in Game1.hm){1}).
-    - auto => />.
-    sp; seq 1 1: (#pre /\ tk{1} = r{2}); 1: by auto => />.
-    auto => />.
-
-  + proc; inline.
-    sp 2 2; match = => // sk.
-    match = => //.
-    seq 1 1: (#pre /\ ={kp}); 1: by auto.
-    sp 1 1; if => //.
-    sp. seq 1 1: (#pre /\ tk{1} = r0{2}); 1: by auto => />.
-    auto => />.
-
-  + proc; inline.
-    sp 1 1; match = => // st.
-    match = => // st' pt ir.
-    sp. seq 1 1: (#pre /\ tk{1} = r0{2}); 1: by auto.
-    auto => />.
-
-  + auto => /#.
-
-transitivity*  {2} { r <@ ROc.IdealAll.MainD(Red_ROM_ideal(A), ROSc.RO_Pair(ROSc.I1.RO,ROSc.I2.RO)).distinguish(); };
-  1: by call (ROSc.RO_split (Red_ROM_ideal(A))).
-
-inline; wp.
-call (: ={b0, servers, c_smap, s_smap, tested, kp_set, bad}(Red_ROM_ideal.AKE_O, Game2) /\ Game2.h1m{2} = ROSc.I1.RO.m{1} /\ Game2.h2m{2} = ROSc.I2.RO.m{1}
-          /\ forall x, x \in ROSc.I1.RO.m{1} <=> x \in ROSc.I2.RO.m{1}); 
-    try sim />.
-
-+ proc; inline.
-  case ((x \in Game1.hm){1}).
-  - auto => />. smt(mem_set).
-  sp; seq 1 1: (#pre /\ r{1} = t{2}); 1: by auto => />.
-  auto => />.
-  smt(mem_set).
-
-+ proc; inline. 
   sp 2 2; match = => // sk.
   match = => //.
   seq 1 1: (#pre /\ ={kp}); 1: by auto.
@@ -1061,28 +913,28 @@ rewrite !mem_filter !domE -eqsm.
 by case: (sml.[x])=> /> [] @/c_clear_k /#.
 qed.
 
-lemma game2_delay_real &m: Pr[E_GAKE(Game2, A).run(false) @ &m : res] = Pr[ROSc.I2.MainD(Red_ROM2_real(A, ROSc.I1.RO), ROSc.I2.LRO).distinguish() @ &m : res].
+lemma game2_delay bit &m: Pr[E_GAKE(Game2, A).run(bit) @ &m : res] = Pr[ROSc.I2.MainD(Red_ROM2(A, ROSc.I1.RO), ROSc.I2.LRO).distinguish(bit) @ &m : res].
 proof. 
-byequiv (: ={glob A, glob Red_ROM2_real} /\ arg{1} = false ==> _)  => //.
+byequiv (: ={glob A, glob Red_ROM2} /\ arg{1} = bit /\ arg{2} = bit ==> _)  => //.
 proc*.
 
-rewrite equiv [{2} 1 -(ROSc.I2.FullEager.RO_LRO (Red_ROM2_real(A, ROSc.I1.RO)) _)]; 2: by move => _; exact dkey_ll.
+rewrite equiv [{2} 1 -(ROSc.I2.FullEager.RO_LRO (Red_ROM2(A, ROSc.I1.RO)) _)]; 2: by move => _; exact dkey_ll.
 
 + inline; wp.
-  call (: ={b0, hm, servers, tested, kp_set, bad, hq, tq, badq}(Game2, Red_ROM2_real.AKE_O) /\ Game2.b0{1} = false
+  call (: ={b0, hm, servers, tested, kp_set, bad, hq, tq, badq}(Game2, Red_ROM2.AKE_O)
           /\ Game2.h1m{1} = ROSc.I1.RO.m{2} /\ Game2.h2m{1} = ROSc.I2.RO.m{2}
-          /\ (forall h, omap (fun v => c_clear_k v) Game2.c_smap.[h]{1} = Red_ROM2_real.AKE_O.c_smap.[h]{2})
-          /\ (forall h, omap (fun v => s_clear_k v) Game2.s_smap.[h]{1} = Red_ROM2_real.AKE_O.s_smap.[h]{2})
+          /\ (forall h, omap (fun v => c_clear_k v) Game2.c_smap.[h]{1} = Red_ROM2.AKE_O.c_smap.[h]{2})
+          /\ (forall h, omap (fun v => s_clear_k v) Game2.s_smap.[h]{1} = Red_ROM2.AKE_O.s_smap.[h]{2})
           /\ (forall i st pt ir, Game2.c_smap{1}.[i] = Some (Pending st pt ir) 
                 => (exists b, ir = (b, false, false)))
           /\ (forall i st pt ir, Game2.s_smap{1}.[i] = Some (Pending st pt ir) 
                 => ir = (false, false, false))
           /\ (forall i st pt k ir, Game2.c_smap{1}.[i] = Some (Accepted st pt k ir)
-                => (exists k', Red_ROM2_real.AKE_O.c_smap{2}.[i] = Some (Accepted st pt k' ir))
+                => (exists k', Red_ROM2.AKE_O.c_smap{2}.[i] = Some (Accepted st pt k' ir))
                    /\ ((oget pt.`2).`1 ^ st.`4, st.`2 ^ st.`4, st.`1, st.`3, (oget pt.`2).`1) \in ROSc.I2.RO.m{2}
                    /\ k = oget ROSc.I2.RO.m{2}.[((oget pt.`2).`1 ^ st.`4, st.`2 ^ st.`4, st.`1, st.`3, (oget pt.`2).`1)])
           /\ (forall i st pt k ir, Game2.s_smap{1}.[i] = Some (Accepted st pt k ir)
-                => (exists k', Red_ROM2_real.AKE_O.s_smap{2}.[i] = Some (Accepted st pt k' ir))
+                => (exists k', Red_ROM2.AKE_O.s_smap{2}.[i] = Some (Accepted st pt k' ir))
                    /\ (pt.`1 ^ oget st.`3, pt.`1 ^ st.`2, st.`1, pt.`1, (oget pt.`2).`1) \in ROSc.I2.RO.m{2}
                    /\ k = oget ROSc.I2.RO.m{2}.[(pt.`1 ^ oget st.`3, pt.`1 ^ st.`2, st.`1, pt.`1, (oget pt.`2).`1)])
           /\ forall x, x \in ROSc.I1.RO.m{2} <=> x \in ROSc.I2.RO.m{2}); last first.
@@ -1150,14 +1002,14 @@ oget ROSc.I2.RO.m{2}.[m3{2}.`1 ^ sk_ce{2}, pk_b{2} ^ sk_ce{2}, b{2}, pk_ce{2}, m
     if=> //. 
     + auto=> /> &1 &2.
       case _: (Game2.c_smap{1}.[i{2}])=> /> c_smap1_i.
-      case _: (Red_ROM2_real.AKE_O.c_smap.[i]{2})=> /> c_smap2_i.
+      case _: (Red_ROM2.AKE_O.c_smap.[i]{2})=> /> c_smap2_i.
       move=> c_clear s_clear inv1 inv2 inv3 inv4 eq_dom mem_ro.
       move: c_smap2_i; rewrite -c_clear.
       rewrite c_smap1_i=> />. 
       smt(get_setE).
     + auto=> /> &1 &2.
       case _: (Game2.c_smap{1}.[i{2}])=> /> c_smap1_i.
-      case _: (Red_ROM2_real.AKE_O.c_smap.[i]{2})=> /> c_smap2_i.
+      case _: (Red_ROM2.AKE_O.c_smap.[i]{2})=> /> c_smap2_i.
       move=> c_clear s_clear inv1 inv2 inv3 eq_dom mem_ro.
       move: c_smap2_i; rewrite -c_clear.
       rewrite c_smap1_i=> />.
@@ -1175,7 +1027,7 @@ oget ROSc.I2.RO.m{2}.[m3{2}.`1 ^ sk_ce{2}, pk_b{2} ^ sk_ce{2}, b{2}, pk_ce{2}, m
     rcondf{2} ^if; 1: by auto => /#.
     auto => /> &1 &2.
     case _: (Game2.c_smap{1}.[i{2}])=> /> c_smap1_i.
-    case _: (Red_ROM2_real.AKE_O.c_smap.[i]{2})=> /> c_smap2_i.
+    case _: (Red_ROM2.AKE_O.c_smap.[i]{2})=> /> c_smap2_i.
     move=> c_clear s_clear inv1 inv2 inv3 inv4 eq_dom _ k _. 
     smt(get_setE mem_set).
 
@@ -1191,7 +1043,7 @@ oget ROSc.I2.RO.m{2}.[m3{2}.`1 ^ sk_ce{2}, pk_b{2} ^ sk_ce{2}, b{2}, pk_ce{2}, m
     rcondf{2} ^if; 1: by auto => /#.
     auto => /> &1 &2.
     case _: (Game2.s_smap{1}.[(b, j){2}])=> /> s_smap1_i.
-    case _: (Red_ROM2_real.AKE_O.s_smap.[(b, j)]{2})=> /> s_smap2_i.
+    case _: (Red_ROM2.AKE_O.s_smap.[(b, j)]{2})=> /> s_smap2_i.
     move=> c_clear s_clear inv1 inv2 inv3 inv4 eq_dom _ k _.
     smt(get_setE mem_set).
 
@@ -1249,212 +1101,12 @@ oget ROSc.I2.RO.m{2}.[m3{2}.`1 ^ sk_ce{2}, pk_b{2} ^ sk_ce{2}, b{2}, pk_ce{2}, m
     if => //.
     + auto => />.
       smt(c_eq_fresh_ck).
-    rcondt{1} ^if; 1: by auto.
-    rcondt{2} ^if; 1: by auto.
-    auto => />.   auto => /> &1 &2 *.
-    split. smt(get_setE). move => *.
-    split. smt(get_setE).
-    split. smt(get_setE).
-    split. smt(get_setE).
-    smt(get_setE).
-
-  - proc; inline.
-    sp; if => //; sp; match => //.
-    + smt().
-    + smt().
-    move => stl str.
-    match => //; 1..3: smt().
-    move => st'l ptl kl irl st'r ptr kr irr.
     if => //.
     + auto => />.
-      smt(s_eq_fresh_ck).
-    rcondt{1} ^if; 1: by auto.
-    rcondt{2} ^if; 1: by auto.
-    auto => />.
-    smt(get_setE).
-qed.
-
-
-print eq_except.
-
-lemma game2_delay_ideal &m: Pr[E_GAKE(Game2, A).run(true) @ &m : res] = Pr[ROSc.I2.MainD(Red_ROM2_ideal(A, ROSc.I1.RO), ROSc.I2.LRO).distinguish() @ &m : res].
-proof. 
-byequiv (: ={glob A, glob Red_ROM2_ideal} /\ arg{1} = true ==> _)  => //.
-proc*.
-
-rewrite equiv [{2} 1 -(ROSc.I2.FullEager.RO_LRO (Red_ROM2_ideal(A, ROSc.I1.RO)) _)]; 2: by move => _; exact dkey_ll.
-
-inline; wp.
-call (: ={b0, hm, servers, tested, kp_set, bad, hq, tq, badq}(Game2, Red_ROM2_ideal.AKE_O) /\ Game2.b0{1} = true
-          /\ Game2.h1m{1} = ROSc.I1.RO.m{2} /\ Game2.h2m{1} = ROSc.I2.RO.m{2}
-          /\ (forall h, omap (fun v => c_clear_k v) Game2.c_smap.[h]{1} = Red_ROM2_ideal.AKE_O.c_smap.[h]{2})
-          /\ (forall h, omap (fun v => s_clear_k v) Game2.s_smap.[h]{1} = Red_ROM2_ideal.AKE_O.s_smap.[h]{2})
-          /\ (forall i st pt ir, Game2.c_smap{1}.[i] = Some (Pending st pt ir) 
-                => (exists b, ir = (b, false, false)))
-          /\ (forall i st pt ir, Game2.s_smap{1}.[i] = Some (Pending st pt ir) 
-                => ir = (false, false, false))
-          /\ (forall i st pt k ir, Game2.c_smap{1}.[i] = Some (Accepted st pt k ir)
-                => (exists k', Red_ROM2_ideal.AKE_O.c_smap{2}.[i] = Some (Accepted st pt k' ir))
-                   /\ ((oget pt.`2).`1 ^ st.`4, st.`2 ^ st.`4, st.`1, st.`3, (oget pt.`2).`1) \in ROSc.I2.RO.m{2}
-                   /\ k = oget ROSc.I2.RO.m{2}.[((oget pt.`2).`1 ^ st.`4, st.`2 ^ st.`4, st.`1, st.`3, (oget pt.`2).`1)])
-          /\ (forall i st pt k ir, Game2.s_smap{1}.[i] = Some (Accepted st pt k ir)
-                => (exists k', Red_ROM2_ideal.AKE_O.s_smap{2}.[i] = Some (Accepted st pt k' ir))
-                   /\ (pt.`1 ^ oget st.`3, pt.`1 ^ st.`2, st.`1, pt.`1, (oget pt.`2).`1) \in ROSc.I2.RO.m{2}
-                   /\ k = oget ROSc.I2.RO.m{2}.[(pt.`1 ^ oget st.`3, pt.`1 ^ st.`2, st.`1, pt.`1, (oget pt.`2).`1)])
-          /\ forall x, x \in ROSc.I1.RO.m{2} <=> x \in ROSc.I2.RO.m{2}); last first.
-  - by auto => />; smt(map_empty emptyE).
-
-  - proc; inline; auto => />; smt(mem_set get_setE).
-
-  - by sim />. 
-  
-  - by sim />.
-
-  - proc; inline.
-    sp; if => //.
-    sp; match.
-    + smt().
-    + smt().
-    + by auto=> />; smt(get_setE).
-    move=> stl str; auto=> />.
-    smt(get_setE).
-
-- proc; inline.
-    sp; match = => // sk.
-    match => //.
-    + smt().
-    + smt().
-    seq 1 1: (#pre /\ ={kp}); 1:by auto.
-    sp 1 1; if => //.
-    swap {1} ^ts<$ @ 1; swap {1} ^ks<$ @ 2.
-    swap {2} ^r0<$ @ 1; swap {2} ^r1<$ @ 2. 
-    seq  2  2: (#pre /\ ts{1} = r0{2} /\ ks{1} = r1{2}); 1: by auto=> />.
-    sp ^if & -1 ^if & -1; if {1} => //.
-      + rcondt {1} ^if; 1: by auto => /#.
-        rcondt {2} ^if; 1: by auto => /#.
-        rcondt {2} ^if; 1: by auto => /#. 
-        auto => /> &1 &2.
-        smt(mem_set get_setE).
-      + rcondf {1} ^if; 1: by auto => /#.
-        rcondf {2} ^if; 1: by auto => /#.
-        rcondf {2} ^if; 1: by auto => /#.
-        auto => /> &1 &2.
-        smt(mem_set get_setE).
-
-  - proc; inline.
-    sp; match => //.
-    + smt().
-    + smt().
-    move=> stl str.
-    match => //; 1..3: smt().
-    move => st'l ptl irl st'r ptr irr.
-    swap {1} ^ts<$ @ 1; swap {1} ^ks<$ @ 2.
-    swap {2} ^r0<$ @ 1; swap {2} ^r1<$ @ 2.
-    seq  2  2: (#pre /\ ts{1} = r0{2} /\ ks{1} = r1{2}); 1: by auto.
-    sp ^if & -1   ^if & -1.
-    seq  ^if{3} & -1   ^if{3} & -1: (#pre /\ ={t_A} /\ sk{2} = witness /\ (x0{2} \in ROSc.I1.RO.m{2}) /\ sk{1} =
-oget ROSc.I2.RO.m{2}.[m3{2}.`1 ^ sk_ce{2}, pk_b{2} ^ sk_ce{2}, b{2}, pk_ce{2}, m3{2}.`1]).
-    + if {1} => //.
-      + rcondt {1} ^if; 1: by auto => /#.
-        rcondt {2} ^if; 1: by auto => /#.
-        rcondt {2} ^if; 1: by auto => /#.
-        by auto=> />; smt(mem_set get_setE).
-      + rcondf {1} ^if; 1: by auto => /#.
-        rcondf {2} ^if; 1: by auto => /#.
-        rcondf {2} ^if; 1: by auto => /#.
-        by auto=> />; smt(mem_set get_setE).
-    if=> //. 
-    + auto=> /> &1 &2.
-      case _: (Game2.c_smap{1}.[i{2}])=> /> c_smap1_i.
-      case _: (Red_ROM2_ideal.AKE_O.c_smap.[i]{2})=> /> c_smap2_i.
-      move=> c_clear s_clear inv1 inv2 inv3 inv4 eq_dom mem_ro.
-      move: c_smap2_i; rewrite -c_clear.
-      rewrite c_smap1_i=> />. 
       smt(get_setE).
-    + auto=> /> &1 &2.
-      case _: (Game2.c_smap{1}.[i{2}])=> /> c_smap1_i.
-      case _: (Red_ROM2_ideal.AKE_O.c_smap.[i]{2})=> /> c_smap2_i.
-      move=> c_clear s_clear inv1 inv2 inv3 eq_dom mem_ro.
-      move: c_smap2_i; rewrite -c_clear.
-      rewrite c_smap1_i=> />.
-      by smt(get_setE).
-
-- proc; inline.
-    sp; match=> //.
-    + smt().
-    + smt().
-    move => stl str.
-    match => //; 1..3: smt().
-    move => st'l ptl kl irl st'r ptr kr irr.
-    if => //.
-    + auto=> />. smt(c_eq_partners_ck).
-    rcondf{2} ^if; 1: by auto => /#.
-    auto => /> &1 &2.
-    case _: (Game2.c_smap{1}.[i{2}])=> /> c_smap1_i.
-    case _: (Red_ROM2_ideal.AKE_O.c_smap.[i]{2})=> /> c_smap2_i.
-    move=> c_clear s_clear inv1 inv2 inv3 inv4 eq_dom _ k _. 
-    smt(get_setE mem_set).
-
-  - proc; inline.
-    sp; match=> //.
-    + smt().
-    + smt().
-    move => stl str.
-    match => //; 1..3: smt().
-    move => st'l ptl kl irl st'r ptr kr irr.
-    if => //.
-    + auto=> />. smt(s_eq_partners_ck).
-    rcondf{2} ^if; 1: by auto => /#.
-    auto => /> &1 &2.
-    case _: (Game2.s_smap{1}.[(b, j){2}])=> /> s_smap1_i.
-    case _: (Red_ROM2_ideal.AKE_O.s_smap.[(b, j)]{2})=> /> s_smap2_i.
-    move=> c_clear s_clear inv1 inv2 inv3 inv4 eq_dom _ k _.
-    smt(get_setE mem_set).
-
-- proc; inline.
-    sp; match => //.
-    move => stl str.
-    match = => // kp.
-    if => //.
-    + move => /> &1 &2 hkp _ sstl sstr c_clear s_clear inv1 inv2 inv3 inv4 eq_dom.
-      split.
-      + move => + j - /(_ j). 
-        rewrite !domE -s_clear => />.
-        case : (Game2.s_smap.[b{2}, j]{1}) => />.
-        smt(s_eq_partners_ck). 
-      move => + j - /(_ j). 
-      rewrite !domE -s_clear => />.
-      case : (Game2.s_smap.[b{2}, j]{1}) => />.
-      smt(s_eq_partners_ck).
     auto => />.
-  
-  - proc; inline.
-    sp; match => //.
-    + smt().
-    + smt().
-    move => stl str.
-    match => //; 1..3: smt().
-    + move => st'l ptl irl st'r ptr irr.
-      auto => /> &1 &2 *. 
-      smt(c_eq_origins_ck get_setE mem_set).
-    move => st'l ptl kl irl st'r ptr kr irr.
-    if => //.
-    + smt(c_eq_partners_ck).
-    auto => /> &1 &2.
     smt(get_setE).
 
-- proc; inline.
-    sp; match => //.
-    + smt().
-    + smt().
-    move => stl str.
-    match => //; 1..3: smt().
-    move => st'l ptl kl irl st'r ptr kr irr.
-    if => //.
-    + smt(s_eq_partners_ck).
-    auto => /> &1 &2.
-    smt(get_setE).
-  
   - proc; inline.
     sp; if => //. sp; match => //.
     + smt().
@@ -1462,62 +1114,53 @@ oget ROSc.I2.RO.m{2}.[m3{2}.`1 ^ sk_ce{2}, pk_b{2} ^ sk_ce{2}, b{2}, pk_ce{2}, m
     move => stl str.
     match => //; 1..3: smt().
     move => st'l ptl kl irl st'r ptr kr irr.
-    if => //. 
-    + auto => />.
-      smt(c_eq_fresh_ck).
-    rcondf{1} ^if; 1: by auto.
-    rcondf{2} ^if; 1: by auto.
-    auto => />.
-    smt(get_setE).
-
-  - proc; inline.
-    sp; if => //; sp; match => //.
-    + smt().
-    + smt().
-    move => stl str.
-    match => //; 1..3: smt().
-    move => st'l ptl kl irl st'r ptr kr irr.
     if => //.
     + auto => />.
       smt(s_eq_fresh_ck).
-    rcondf{1} ^if; 1: by auto.
-    rcondf{2} ^if; 1: by auto.
+    if => //.
+    + auto => />.
+      smt(get_setE).
     auto => />.
     smt(get_setE).
 qed.
+
 
 lemma sofar &m: `| Pr[E_GAKE(GAKEb(NTOR_S(RO), NTOR_C(RO), RO), A).run(false) @ &m : res] - Pr[E_GAKE(GAKEb(NTOR_S(RO), NTOR_C(RO), RO), A).run(true) @ &m : res]|
-  <= `|Pr[ROSc.I2.MainD(Red_ROM2_real(A, ROSc.I1.RO), ROSc.I2.LRO).distinguish() @ &m : res] - Pr[ROSc.I2.MainD(Red_ROM2_ideal(A, ROSc.I1.RO), ROSc.I2.LRO).distinguish() @ &m : res]|
+  <= `|Pr[ROSc.I2.MainD(Red_ROM2(A, ROSc.I1.RO), ROSc.I2.LRO).distinguish(false) @ &m : res] - Pr[ROSc.I2.MainD(Red_ROM2(A, ROSc.I1.RO), ROSc.I2.LRO).distinguish(true) @ &m : res]|
       + 2%r * ((q_is + q_m1 + q_m2) ^ 2)%r * mu1 dkp (mode dkp).
 proof.   
 rewrite !(gake_game0 _).
 apply (StdOrder.RealOrder.ler_trans 
         (`|Pr[E_GAKE(Game1, A).run(false) @ &m : res] - Pr[E_GAKE(Game1, A).run(true) @ &m : res]| + 2%r * ((q_is + q_m1 + q_m2) ^ 2)%r * mu1 dkp (mode dkp))).
 + smt(game0_game1 game0_bad).
-by rewrite !(game1_game2 _) game2_delay_real game2_delay_ideal.
+by rewrite !(game1_game2 _) !game2_delay.
 qed. 
 
 
 
-lemma interestingbit &m: `|Pr[ROSc.I2.MainD(Red_ROM2_real(A, ROSc.I1.RO), ROSc.I2.LRO).distinguish() @ &m : res] - Pr[ROSc.I2.MainD(Red_ROM2_ideal(A, ROSc.I1.RO), ROSc.I2.LRO).distinguish() @ &m : res]| <= Pr[ROSc.I2.MainD(Red_ROM2_real(A, ROSc.I1.RO), ROSc.I2.LRO).distinguish() @ &m : Red_ROM2_real.AKE_O.badq].
+lemma interestingbit &m: `|Pr[ROSc.I2.MainD(Red_ROM2(A, ROSc.I1.RO), ROSc.I2.LRO).distinguish(false) @ &m : res] - Pr[ROSc.I2.MainD(Red_ROM2(A, ROSc.I1.RO), ROSc.I2.LRO).distinguish(true) @ &m : res]| <= Pr[ROSc.I2.MainD(Red_ROM2(A, ROSc.I1.RO), ROSc.I2.LRO).distinguish(false) @ &m : Red_ROM2.AKE_O.badq].
 proof.
 rewrite StdOrder.RealOrder.distrC.
-byequiv (: _ ==> _) : Red_ROM2_ideal.AKE_O.badq => //; first last.
+byequiv (: _ ==> _) : Red_ROM2.AKE_O.badq => //; first last.
 + smt().
 symmetry; proc; inline.
 wp.
-call (: Red_ROM2_ideal.AKE_O.badq
-      , ={servers, c_smap, s_smap, tested, kp_set, hm, bad, hq, tq, badq}(Red_ROM2_real.AKE_O, Red_ROM2_ideal.AKE_O)
-        /\ ROSc.I1.RO.m{1} = ROSc.I1.RO.m{2} /\ (Red_ROM2_real.AKE_O.tq{1} = None => ={ROSc.I2.RO.m})
-        /\ (forall x, Red_ROM2_real.AKE_O.tq{1} = Some x => eq_except (pred1 x) ROSc.I2.RO.m{1} ROSc.I2.RO.m{2})
-        /\ (Red_ROM2_real.AKE_O.tested{1} = false => Red_ROM2_real.AKE_O.tq{1} = None)
-        /\ (forall i st pt k ir, Red_ROM2_ideal.AKE_O.c_smap{2}.[i] = Some (Accepted st pt k ir) /\ get_ir_test (oget Red_ROM2_ideal.AKE_O.c_smap{2}.[i]) <> true
-                => Some ((oget pt.`2).`1 ^ st.`4, st.`2 ^ st.`4, st.`1, st.`3, (oget pt.`2).`1) <> Red_ROM2_ideal.AKE_O.tq{2})
-        /\ (forall i st pt k ir, Red_ROM2_ideal.AKE_O.s_smap{2}.[i] = Some (Accepted st pt k ir) /\ get_ir_test (oget Red_ROM2_ideal.AKE_O.s_smap{2}.[i]) <> true
-                => Some (pt.`1 ^ oget st.`3, pt.`1 ^ st.`2, st.`1, pt.`1, (oget pt.`2).`1) <> Red_ROM2_ideal.AKE_O.tq{2})
-        /\ Red_ROM2_real.AKE_O.b0{1} = false /\ Red_ROM2_ideal.AKE_O.b0{2} = true
+call (: Red_ROM2.AKE_O.badq
+      , ={servers, c_smap, s_smap, tested, kp_set, hm, bad, hq, tq, badq}(Red_ROM2.AKE_O, Red_ROM2.AKE_O)
+        /\ ROSc.I1.RO.m{1} = ROSc.I1.RO.m{2} /\ (Red_ROM2.AKE_O.tq{1} = None => ={ROSc.I2.RO.m})
+        /\ (forall x, Red_ROM2.AKE_O.tq{1} = Some x => eq_except (pred1 x) ROSc.I2.RO.m{1} ROSc.I2.RO.m{2})
+        /\ (Red_ROM2.AKE_O.tested{1} = false => Red_ROM2.AKE_O.tq{1} = None)
+      (*  /\ (Red_ROM2.AKE_O.tq{1} <> None => oget Red_ROM2.AKE_O.tq{1} \in ROSc.I2.RO.m{1}) *)
+        /\ (forall i st pt k ir, Red_ROM2.AKE_O.c_smap{2}.[i] = Some (Accepted st pt k ir) /\ get_ir_test (oget Red_ROM2.AKE_O.c_smap{2}.[i]) <> true
+                => Some ((oget pt.`2).`1 ^ st.`4, st.`2 ^ st.`4, st.`1, st.`3, (oget pt.`2).`1) <> Red_ROM2.AKE_O.tq{2})
+        /\ (forall i st pt k ir, Red_ROM2.AKE_O.s_smap{2}.[i] = Some (Accepted st pt k ir) /\ get_ir_test (oget Red_ROM2.AKE_O.s_smap{2}.[i]) <> true
+                => Some (pt.`1 ^ oget st.`3, pt.`1 ^ st.`2, st.`1, pt.`1, (oget pt.`2).`1) <> Red_ROM2.AKE_O.tq{2})
+        /\ (forall i st pt k ir, Red_ROM2.AKE_O.c_smap{2}.[i] = Some (Accepted st pt k ir) 
+                => forall i' k' ir', Red_ROM2.AKE_O.c_smap{2}.[i'] = Some (Accepted st pt k' ir') 
+                => i = i')
+        /\ Red_ROM2.AKE_O.b0{1} = false /\ Red_ROM2.AKE_O.b0{2} = true
         /\ (forall x, x \in ROSc.I2.RO.m{1} <=> x \in ROSc.I2.RO.m{2})
-      , ={badq}(Red_ROM2_real.AKE_O, Red_ROM2_ideal.AKE_O)) => //; try sim />.
+      , ={badq}(Red_ROM2.AKE_O, Red_ROM2.AKE_O)) => //; try sim />.
 
 - exact A_ll.
 
@@ -1527,18 +1170,18 @@ call (: Red_ROM2_ideal.AKE_O.badq
   + auto => /> &1 &2 badqr hqr *.
     split. move => *. smt(get_setE).
     move => *. split. smt(get_setE).
-    move => *. case (Red_ROM2_ideal.AKE_O.tq{2} = None) => ?; 1: by smt().
-    have: (oget Red_ROM2_ideal.AKE_O.tq{2} \notin hqr `|` fset1 x{2}); 1: by smt().
+    move => *. case (Red_ROM2.AKE_O.tq{2} = None) => ?; 1: by smt().
+    have: (oget Red_ROM2.AKE_O.tq{2} \notin hqr `|` fset1 x{2}); 1: by smt().
     move => ?.
-    have: oget Red_ROM2_ideal.AKE_O.tq{2} <> x{2}; 1: by smt(@FSet).
+    have: oget Red_ROM2.AKE_O.tq{2} <> x{2}; 1: by smt(@FSet).
     by smt().
   auto => /> &1 &2 badqr hqr *.
   split; 1: by smt(get_setE).
   move => *. split; 1: by smt(get_setE).
-  move => *. case (Red_ROM2_ideal.AKE_O.tq{2} = None) => ?; 1: by smt().
-  have: (oget Red_ROM2_ideal.AKE_O.tq{2} \notin hqr `|` fset1 x{2}); 1: by smt().
+  move => *. case (Red_ROM2.AKE_O.tq{2} = None) => ?; 1: by smt().
+  have: (oget Red_ROM2.AKE_O.tq{2} \notin hqr `|` fset1 x{2}); 1: by smt().
   move => ?.
-  have: oget Red_ROM2_ideal.AKE_O.tq{2} <> x{2}; 1: by smt(@FSet).
+  have: oget Red_ROM2.AKE_O.tq{2} <> x{2}; 1: by smt(@FSet).
   by smt().
 - move => &2 badq; proc*; inline. auto => />. 
   rewrite dkey_ll dtag_ll //=. smt().
@@ -1557,7 +1200,6 @@ call (: Red_ROM2_ideal.AKE_O.badq
   proc; auto => />.
 - move => &1. 
   proc; auto => />. 
-
 
 - proc; inline.
   sp; if => //.
@@ -1585,12 +1227,15 @@ call (: Red_ROM2_ideal.AKE_O.badq
   sp 1 1; if => //.
   sp; seq 1 1: (#pre /\ ={r0}); 1: by auto=> />.
   if => //.  
-  + auto => /> &1 &2 kps bad stm _ stnn _ neqb inv1 inv2 inv3 inv4 inv5 inv6 fresh notinm i0 st pt k ir.
+  + auto => /> &1 &2 kps bad stm _ stnn _ neqb inv1 inv2 inv3 inv4 inv5 inv6 inv7 inv8 fresh notinm i0 st pt k ir.
+    case (Red_ROM2.AKE_O.tq{2} = None).
+    + smt().
+    
     case (i0 = (b, j){2}) => eqi.
     + rewrite eqi get_set_sameE //=. rewrite get_setE //=.
       admit. (* need that traces are unique and there is no collision with tq *)
     by rewrite get_set_neqE //#.
-  auto => /> &1 &2 kps bad stm _ stnn _ neqb inv1 inv2 inv3 inv4 inv5 inv6 fresh inm i0 st pt k ir.
+  auto => /> &1 &2 kps bad stm _ stnn _ neqb inv1 inv2 inv3 inv4 inv5 inv6 inv7 fresh inm i0 st pt k ir.
   case (i0 = (b, j){2}) => eqi.
   + rewrite eqi get_set_sameE //=.
     admit. (* need that traces are unique and there is no collision with tq *)
